@@ -1,0 +1,10 @@
+/-
+`sys_wait` meets its specification, given `argaddr` and `kwait`.
+-/
+import Xv6.ProofSysWait
+
+namespace Xv6
+
+theorem SysWait (AA : ARGADDR) (KW : KWAIT) : SYSWAIT := sys_wait_proof AA KW
+
+end Xv6
